nested both

Cm/Pi/Infer.lean
@@ -330,9 +330,27 @@ def infer_eq.inject_future_infer' : Expr :=
               Expr.id))
           (q' q' infer.assert_well_typed_unsafe)))))))))
 
+example : (:: (q' both) (::
+              (q' q' const)
+              Expr.id)) = mk_both' 1 (:: (q' q' const) Expr.id) := rfl
+
+def infer_eq.inject_future_infer'' : Expr :=
+  mk_both' 0 (:: (q' both) (::
+    (q' q' both)
+    (:: (q' both) (::
+      (q' q' (quote apply))
+        (:: (q' both) (::
+          (q' q' both)
+          (:: (q' both) (::
+            (:: (q' both) (::
+              (q' q' const)
+              Expr.id))
+          (q' q' infer.assert_well_typed_unsafe)))))))))
+
 example : (quote (quote infer.assert_well_typed_unsafe)) = (q' q' infer.assert_well_typed_unsafe) := rfl
 
 example : infer_eq.inject_future_infer = infer_eq.inject_future_infer' := rfl
+example : infer_eq.inject_future_infer = infer_eq.inject_future_infer'' := rfl
 
 /-
 Checks that the eq maps have the same type,
